Fix Sequential Behavior

src/sequential/SequentialBehavior.v
@@ -14,7 +14,7 @@ From PromisingLib Require Import Loc.
 Require Import Event.
 Require Import List.
 
-Require Import Debt.
+Require Import SequentialDef.
 
 Set Implicit Arguments.
 
@@ -41,161 +41,49 @@ Proof.
 Qed.
 
 
-Module SeqEvent.
-  Variant t: Set :=
-  | read
-      (loc: Loc.t) (val: Const.t) (ord: Ordering.t)
-      (d: diffs) (c: SeqCell.t)
-  | write
-      (loc: Loc.t) (val: Const.t) (ord: Ordering.t)
-      (d: diffs) (c: SeqCell.t) (m_released: option SeqMemory.t)
-  | update
-      (loc: Loc.t) (valr: Const.t) (valw: Const.t) (ordr: Ordering.t) (ordw: Ordering.t)
-      (d: diffs) (c: SeqCell.t) (m_released: option SeqMemory.t)
-  | fence
-      (ordr: Ordering.t) (ordw: Ordering.t)
-      (d: diffs) (m_released: option SeqMemory.t)
-  | syscall
-      (e: Event.t)
-      (d: diffs) (f: Flags.t) (m_released: SeqMemory.t)
-  .
-
-  Definition get_event (e: ProgramEvent.t) (m: SeqMemory.t) (d: diffs) (m_released: option SeqMemory.t): option t :=
-    match e with
-    | ProgramEvent.silent | ProgramEvent.failure => None
-    | ProgramEvent.read loc val ord =>
-      Some (read loc val ord d (m loc))
-    | ProgramEvent.write loc val ord =>
-      let m_released := if Ordering.le Ordering.strong_relaxed ord
-                        then m_released
-                        else None in
-      Some (write loc val ord d (m loc) m_released)
-    | ProgramEvent.update loc valr valw ordr ordw =>
-      let m_released := if Ordering.le Ordering.strong_relaxed ordw
-                        then m_released
-                        else None in
-      Some (update loc valr valw ordr ordw d (m loc) m_released)
-    | ProgramEvent.fence ordr ordw =>
-      let m_released := if Ordering.le Ordering.strong_relaxed ordw
-                        then m_released
-                        else None in
-      Some (fence ordr ordw d m_released)
-    | ProgramEvent.syscall e =>
-      let f := (SeqMemory.flags m) in
-      match m_released with
-      | None => None
-      | Some m_released =>
-        Some (syscall e d f m_released)
-      end
-    end.
-
-  Variant le: t -> t -> Prop :=
-  | le_read
-      loc val ord d c0 c1
-      (CELL: SeqCell.le c0 c1)
-    :
-      le (read loc val ord d c0) (read loc val ord d c1)
-  | le_write
-      loc val ord d c0 c1 m0 m1
-      (CELL: SeqCell.le c0 c1)
-      (RELEASED: option_rel SeqMemory.le m0 m1)
-    :
-      le (write loc val ord d c0 m0) (write loc val ord d c1 m1)
-  | le_update
-      loc valr valw ordr ordw d c0 c1 m0 m1
-      (CELL: SeqCell.le c0 c1)
-      (RELEASED: option_rel SeqMemory.le m0 m1)
-    :
-      le (update loc valr valw ordr ordw d c0 m0) (update loc valr valw ordr ordw d c1 m1)
-  | le_fence
-      ordr ordw d m0 m1
-      (RELEASED: option_rel SeqMemory.le m0 m1)
-    :
-      le (fence ordr ordw d m0) (fence ordr ordw d m1)
-  | le_syscall
-      e d f0 f1 m0 m1
-      (RELEASED: SeqMemory.le m0 m1)
-    :
-      le (syscall e d f0 m0) (syscall e d f1 m1)
-  .
-
-  Program Instance le_PreOrder: PreOrder le.
-  Next Obligation.
-  Proof.
-    ii. destruct x; econs; refl.
-  Qed.
-  Next Obligation.
-  Proof.
-    ii. inv H; inv H0; econs; etrans; eauto.
-  Qed.
-End SeqEvent.
-
-
 Module SeqTrace.
-  Variant t: Set :=
-  | term (es: list SeqEvent.t) (m: SeqMemory.t)
-  | partial (es: list SeqEvent.t) (f: Flags.t)
-  | ub (es: list SeqEvent.t)
+  Variant output: Set :=
+  | term (m: SeqMemory.t)
+  | partial (f: Flags.t)
+  | ub
   .
 
-  Definition cons (e: SeqEvent.t) (tr: t): t :=
-    match tr with
-    | term es m => term (e::es) m
-    | partial es f => partial (e::es) f
-    | ub es => ub (e::es)
-    end.
-
-  Definition cons_opt (e: option SeqEvent.t) (tr: t): t :=
-    match e with
-    | Some e => cons e tr
-    | None => tr
-    end.
+  Definition t: Type := list (ProgramEvent.t * SeqEvent.input * SeqEvent.output) * output.
 
   Variant le: t -> t -> Prop :=
   | le_term
-      es_src es_tgt m_src m_tgt
-      (EVENTS: Forall2 SeqEvent.le es_tgt es_src)
+      es m_src m_tgt
       (MEMORY: SeqMemory.le m_tgt m_src)
     :
-      le (term es_tgt m_tgt) (term es_src m_src)
+      le (es, term m_tgt) (es, term m_src)
   | le_pterm
       es_src es_tgt f_src f_tgt
-      (EVENTS: exists es_hd es_tl,
-          (<<APP: es_src = es_hd ++ es_tl>>) /\
-          (<<FORALL: Forall2 SeqEvent.le es_tgt es_hd>>))
+      (EVENTS: exists es, es_tgt = es_src ++ es)
       (FLAGS: Flags.le f_tgt f_src)
     :
-      le (partial es_tgt f_tgt) (partial es_src f_src)
+      le (es_tgt, partial f_tgt) (es_src, partial f_src)
   | le_ub
-      es_src tr_tgt
+      es tr_tgt
     :
-      le tr_tgt (ub es_src)
+      le tr_tgt (es, ub)
   .
 
   Program Instance le_PreOrder: PreOrder le.
   Next Obligation.
   Proof.
-    ii. destruct x.
-    { econs 1; refl. }
-    { econs 2; [|refl]. exists es, []. splits; [|refl].
+    ii. destruct x as [? []].
+    { econs. refl. }
+    { econs 2; [|refl]. exists [].
       rewrite app_nil_r. auto. }
     { econs 3. }
   Qed.
   Next Obligation.
   Proof.
     ii. inv H; inv H0.
-    { econs 1; eauto.
-      { etrans; eauto. }
-      { etrans; eauto. }
-    }
+    { econs 1; eauto. etrans; eauto. }
     { econs 3. }
-    { des; subst.
-      eapply Forall2_app_inv_l in FORALL. des; subst.
-      econs 2.
-      { eexists l1', (l2' ++ es_tl). splits.
-        { rewrite app_assoc. auto. }
-        { etrans; eauto. }
-      }
+    { des; subst. econs 2.
+      { eexists. rewrite app_assoc. eauto. }
       { etrans; eauto. }
     }
     { econs 3. }
@@ -227,16 +115,16 @@ Section LANG.
       st m p o
       (TERMINAL: lang.(Language.is_terminal) st)
     :
-      behavior (SeqThread.mk (SeqState.mk _ st m) p o) (SeqTrace.term [] m)
+      behavior (SeqThread.mk (SeqState.mk _ st m) p o) ([], SeqTrace.term m)
   | behavior_partial
       st m p o
     :
-      behavior (SeqThread.mk (SeqState.mk _ st m) p o) (SeqTrace.partial [] (SeqMemory.flags m))
+      behavior (SeqThread.mk (SeqState.mk _ st m) p o) ([], SeqTrace.partial (SeqMemory.flags m))
   | behavior_ub
       st m p o
       (FAILURE: SeqThread.failure (SeqThread.mk (SeqState.mk _ st m) p o))
     :
-      behavior (SeqThread.mk (SeqState.mk _ st m) p o) (SeqTrace.ub [])
+      behavior (SeqThread.mk (SeqState.mk _ st m) p o) ([], SeqTrace.ub)
   | behavior_na_step
       th0 th1 tr
       (STEP: SeqThread.na_step MachineEvent.silent th0 th1)
@@ -244,12 +132,11 @@ Section LANG.
     :
       behavior th0 tr
   | behavior_at_step
-      th0 th1 pe d m_released e tr
-      (STEP: SeqThread.at_step pe d m_released th0 th1)
-      (EVENT: SeqEvent.get_event pe th0.(SeqThread.state).(SeqState.memory) d m_released = Some e)
-      (BEHAVIOR: behavior th1 tr)
+      e i o th0 th1 es st
+      (STEP: SeqThread.at_step e i o th0 th1)
+      (BEHAVIOR: behavior th1 (es, st))
     :
-      behavior th0 (SeqTrace.cons e tr)
+      behavior th0 ((e, i, o)::es, st)
   .
 End LANG.
 
@@ -257,10 +144,10 @@ Definition refine
            (lang_tgt lang_src: language)
            (st_tgt: lang_tgt.(Language.state)) (st_src: lang_src.(Language.state))
   : Prop :=
-  forall o p vals (WF: Oracle.wf o),
+  forall o p m (WF: Oracle.wf o),
     SeqTrace.incl
-      (behavior (SeqThread.mk (SeqState.mk _ st_tgt (SeqMemory.init vals)) p o))
-      (behavior (SeqThread.mk (SeqState.mk _ st_src (SeqMemory.init vals)) p o)) .
+      (behavior (SeqThread.mk (SeqState.mk _ st_tgt m) p o))
+      (behavior (SeqThread.mk (SeqState.mk _ st_src m) p o)) .
 End SeqBehavior.
 
 
